platform/ThreadQueues.v
@@ -1,0 +1,236 @@
+Require Import AutoSep Bags Malloc RecPred ThreadQueue.
+Import W_Bag.
+
+Set Implicit Arguments.
+
+
+Module Type S.
+  Variable globalInv : bag -> HProp.
+End S.
+
+Module Make(M : S).
+Import M.
+
+Module M'.
+  Open Scope Sep_scope.
+
+  Definition globalInv (p : W) : hpropB ((settings * state : Type)%type :: nil) :=
+    Ex b, starB (fun p' stn sm => Var0 (stateOut (stn, sm) p')) b * ^[globalInv (b %+ p)].
+End M'.
+
+Module Q := ThreadQueue.Make(M').
+Import Q.
+
+Module Type TQS.
+  Parameter tqs : bag -> HProp.
+
+  Axiom tqs_eq : tqs = starB tq.
+
+  Definition tqs_pick_this_one (_ : W) := tqs.
+
+  Axiom tqs_empty_bwd : Emp ===> tqs empty.
+  Axiom tqs_add_bwd : forall ts t, tqs ts * tq t ===> tqs (ts %+ t).
+  Axiom tqs_del_fwd : forall ts t, t %in ts -> tqs_pick_this_one t ts ===> tq t * tqs (ts %- t).
+  Axiom tqs_del_bwd : forall ts t, t %in ts -> tqs (ts %- t) * tq t ===> tqs ts.
+End TQS.
+
+Module Tqs : TQS.
+  Open Scope Sep_scope.
+
+  Definition tqs := starB tq.
+
+  Theorem tqs_eq : tqs = starB tq.
+    auto.
+  Qed.
+
+  Definition tqs_pick_this_one (_ : W) := tqs.
+
+  Theorem tqs_empty_bwd : Emp ===> tqs empty.
+    apply starB_empty_bwd.
+  Qed.
+
+  Theorem tqs_add_bwd : forall ts t, tqs ts * tq t ===> tqs (ts %+ t).
+    apply starB_add_bwd.
+  Qed.
+
+  Theorem tqs_del_fwd : forall ts t, t %in ts -> tqs_pick_this_one t ts ===> tq t * tqs (ts %- t).
+    apply starB_del_fwd.
+  Qed.
+
+  Theorem tqs_del_bwd : forall ts t, t %in ts -> tqs (ts %- t) * tq t ===> tqs ts.
+  Admitted.
+End Tqs.
+
+Import Tqs.
+Export Tqs.
+
+Definition hints : TacPackage.
+  prepare tqs_del_fwd (tqs_empty_bwd, tqs_add_bwd).
+Defined.
+
+Definition starting (pc : W) (ss : nat) : HProp := fun s m =>
+  (ExX (* pre *) : settings * state, Cptr pc #0
+    /\ [| semp m |]
+    /\ Al st : settings * state, Al vs, Al ts,
+      ![ ^[locals ("rp" :: "sc" :: nil) vs ss st#Sp * tqs ts * globalInv ts * mallocHeap 0] ] st
+      ---> #0 st)%PropX.
+
+Lemma starting_elim : forall specs pc ss P stn st,
+  interp specs (![ starting pc ss * P ] (stn, st))
+  -> (exists pre, specs pc = Some (fun x => pre x)
+    /\ interp specs (![ P ] (stn, st))
+    /\ forall stn_st vs ts, interp specs (![ locals ("rp" :: "sc" :: nil) vs ss stn_st#Sp
+      * tqs ts * globalInv ts * mallocHeap 0 ] stn_st
+    ---> pre stn_st)%PropX).
+  cptr.
+  generalize (split_semp _ _ _ H0 H); intros; subst; auto.
+  rewrite <- sepFormula_eq; descend; step auto_ext.
+Qed.
+
+
+Definition allocS : spec := SPEC reserving 15
+  Al ts,
+  PRE[_] tqs ts * mallocHeap 0
+  POST[R] tqs (ts %+ R) * mallocHeap 0.
+
+Definition spawnS : spec := SPEC("q", "pc", "ss") reserving 25
+  Al ts,
+  PRE[V] [| V "q" %in ts |] * [| V "ss" >= $2 |]
+    * tqs ts * starting (V "pc") (wordToNat (V "ss") - 2) * mallocHeap 0
+  POST[_] tqs ts * mallocHeap 0.
+
+Definition m := bimport [[ "threadq"!"init" @ [Q.initS], "threadq"!"spawn" @ [Q.spawnS] ]]
+  bmodule "threadqs" {{
+    bfunction "alloc"("r") [allocS]
+      "r" <-- Call "threadq"!"init"()
+      [PRE[_, R] tq R
+       POST[R'] tq R'];;
+      Return "r"
+    end with bfunction "spawn"("q", "pc", "ss") [spawnS]
+      Call "threadq"!"spawn"("q", "pc", "ss")
+      [PRE[_] Emp
+       POST[_] Emp];;
+      Return 0
+    end
+  }}.
+
+Hint Extern 1 (@eq W _ _) => words.
+
+Ltac t := sep hints; auto.
+
+Theorem ok : moduleOk m.
+  vcgen.
+
+  t.
+  t.
+  t.
+  t.
+  t.
+  t.
+  t.
+  t.
+
+  t.
+  t.
+  t.
+  t.
+
+  post; evaluate hints; descend.
+  change (tqs x0) with (tqs_pick_this_one (sel x2 "q") x0) in H7.
+  toFront ltac:(fun P => match P with
+                           | starting _ _ => idtac
+                         end) H7; apply starting_elim in H7; post.
+  toFront_conc ltac:(fun P => match P with
+                                | Q.starting _ _ _ => idtac
+                              end); apply Q.starting_intro; descend.
+  2: step hints.
+  step hints.
+  step hints.
+  descend.
+  apply andL; apply swap; apply injL; intro.
+  unfold ginv, M'.globalInv.
+  autorewrite with sepFormula.
+  match goal with
+    | [ |- interp _ (![?P * exB ?Q * ?R] ?p ---> _)%PropX ] =>
+      apply Imply_trans with (![Ex b, P * Q b * R] p)%PropX
+  end.
+  make_Himp.
+  
+  Lemma get_ex : forall P Q R S,
+    P * Q * R * S ===> R * (P * Q * S).
+    sepLemma.
+  Qed.
+
+  eapply Himp_trans; [ apply get_ex | ].
+  eapply Himp_trans; [ apply Himp_ex_star | ].
+  apply Himp'_ex; intro.
+  apply Himp_ex_c; exists x6.
+
+  Lemma get_ex' : forall P Q R S,
+    R * (P * Q * S) ===> P * Q * R * S.
+    sepLemma.
+  Qed.
+
+  apply get_ex'.
+
+  Lemma ex_out : forall A (P : A -> HProp) p specs,
+    interp specs (![exB P] p ---> Ex x, ![P x] p)%PropX.
+    rewrite sepFormula_eq; unfold sepFormula_def; intros.
+    apply Imply_refl.
+  Qed.
+
+  eapply Imply_trans; [ apply ex_out | ].
+  apply existsL; intro.
+  eapply Imply_trans; [ | apply H12 ]; clear H12.
+  make_Himp.
+
+  Lemma Himp_star_assoc' : forall P Q R,
+    P * (Q * R) ===> P * Q * R.
+    sepLemma.
+  Qed.
+
+  Lemma get_first : forall P Q R P' Q' R',
+    P ===> P'
+    -> Q * R ===> Q' * R'
+    -> P * Q * R ===> P' * Q' * R'.
+    intros; eapply Himp_trans; [ | apply Himp_star_assoc' ].
+    eapply Himp_trans; [ apply Himp_star_assoc | ].
+    apply Himp_star_frame; auto.
+  Qed.
+
+  autorewrite with sepFormula.
+  apply Himp_star_frame; try apply Himp_refl.
+  apply get_first.
+  sepLemma.
+
+  Lemma blergh : forall P Q R,
+    P * (Q * R) ===> Q * (P * R).
+    sepLemma.
+  Qed.
+
+  eapply Himp_trans; [ apply blergh | ].
+  eapply Himp_trans.
+  apply Himp_star_frame.
+  apply starB_substH_fwd.
+  apply Himp_refl.
+  eapply Himp_trans.
+  apply Himp_star_frame.
+  instantiate (1 := tqs x6).
+  rewrite tqs_eq; apply starB_weaken; intros.
+  unfold Himp, himp; intros.
+  unfold substH, predOut.
+  simpl.
+  rewrite memoryIn_memoryOut; apply Himp_refl.
+  apply Himp_refl.
+  instantiate (1 := x6 %+ sel x2 "q").
+  intro; step hints.
+  step hints.
+  sep hints; auto.
+  apply tqs_del_bwd; auto.
+
+  t.
+  t.
+  t.
+Qed.
+
+End Make.
